refactor(lib/systems/coq_reflect): simplify contexts

lib/systems/coq_reflect/Profint.v
@@ -1,28 +1,23 @@
 Require Import List.
 Import ListNotations.
 
-Polymorphic Inductive rcx : list Type -> Type :=
-| Hole      : rcx nil
-| RAndL A   : rcx A -> Prop -> rcx A
-| RAndR A   : Prop -> rcx A -> rcx A
-| ROrL A    : rcx A -> Prop -> rcx A
-| ROrR A    : Prop -> rcx A -> rcx A
-| RImpL A   : lcx A -> Prop -> rcx A
-| RImpR A   : Prop -> rcx A -> rcx A
-| RAll A B  : (A -> rcx B) -> rcx (A :: B)
-| REx A B   : (A -> rcx B) -> rcx (A :: B)
-with lcx : list Type -> Type :=
-| LAndL A   : lcx A -> Prop -> lcx A
-| LAndR A   : Prop -> lcx A -> lcx A
-| LOrL A    : lcx A -> Prop -> lcx A
-| LOrR A    : Prop -> lcx A -> lcx A
-| LImpL A   : rcx A -> Prop -> lcx A
-| LImpR A   : Prop -> lcx A -> lcx A
-| LAll A B  : (A -> lcx B) -> lcx (A :: B)
-| LEx A B   : (A -> lcx B) -> lcx (A :: B).
+Inductive side : Type := Pos | Neg.
 
-Reserved Notation "R [[ P ]]" (at level 1, format "'[ ' R [[  P  ]] ']'").
-Reserved Notation "L {{ P }}" (at level 1, format "'[ ' L '{{'  P  '}}' ']'").
+Definition flip (side : side) :=
+  match side with Pos => Neg | _ => Pos end.
+
+Polymorphic Inductive ctx : side -> list Type -> Type :=
+| Hole           : ctx Pos nil
+| AndL side Ts   : ctx side Ts -> Prop -> ctx side Ts
+| AndR side Ts   : Prop -> ctx side Ts -> ctx side Ts
+| OrL side Ts    : ctx side Ts -> Prop -> ctx side Ts
+| OrR side Ts    : Prop -> ctx side Ts -> ctx side Ts
+| ImpL side Ts   : ctx (flip side) Ts -> Prop -> ctx side Ts
+| ImpR side Ts   : Prop -> ctx side Ts -> ctx side Ts
+| AllD A side Ts : (A -> ctx side Ts) -> ctx side (A :: Ts)
+| ExD A side Ts  : (A -> ctx side Ts) -> ctx side (A :: Ts).
+
+Reserved Notation "Cx [[ P ]]" (at level 1, format "'[ ' Cx [[  P  ]] ']'").
 
 Fixpoint ho_absract (Ts : list Type) (U : Type) :=
   match Ts return Type with
@@ -31,31 +26,19 @@ Fixpoint ho_absract (Ts : list Type) (U : Type) :=
   end.
 Notation "Ts ▷ U" := (ho_absract Ts U) (at level 100, right associativity).
 
-Fixpoint rcx_place Ts (rcx : rcx Ts) {struct rcx} : (Ts ▷ Prop) -> Prop :=
-  match rcx in (rcx Ts1) return ((Ts1 ▷ Prop) -> Prop) with
-  | Hole          => fun p => p
-  | RAndL _ rcx q => fun p => rcx[[ p ]] /\ q
-  | RAndR _ q rcx => fun p => q /\ rcx[[ p ]]
-  | ROrL _ rcx q  => fun p => rcx[[ p ]] \/ q
-  | ROrR _ q rcx  => fun p => q \/ rcx[[ p ]]
-  | RImpL _ lcx q => fun p => lcx{{ p }} -> q
-  | RImpR _ q rcx => fun p => q -> rcx[[ p ]]
-  | RAll a _ rcx  => fun p => forall (x : a), (rcx x)[[ (p x) ]]
-  | REx a _ rcx   => fun p => exists (x : a), (rcx x)[[ (p x) ]]
+Fixpoint ctx_place side Ts (ctx : ctx side Ts) {struct ctx} : (Ts ▷ Prop) -> Prop :=
+  match ctx in (ctx _ Us) return (Us ▷ Prop) -> Prop with
+  | Hole => fun p => p
+  | AndL _ _ ctx q => fun p => ctx[[ p ]] /\ q
+  | AndR _ _ q ctx => fun p => q /\ ctx[[ p ]]
+  | OrL _ _ ctx q => fun p => ctx[[ p ]] \/ q
+  | OrR _ _ q ctx => fun p => q \/ ctx[[ p ]]
+  | ImpL _ _ ctx q => fun p => ctx[[ p ]] -> q
+  | ImpR _ _ q ctx => fun p => q -> ctx[[ p ]]
+  | AllD A _ _ ctx => fun p => forall (x : A), (ctx x)[[ p x ]]
+  | ExD A _ _ ctx => fun p => exists (x : A), (ctx x)[[ p x ]]
   end
-with lcx_place Ts (lcx : lcx Ts) {struct lcx} : (Ts ▷ Prop) -> Prop :=
-  match lcx in (lcx Ts1) return ((Ts1 ▷ Prop) -> Prop) with
-  | LAndL _ lcx q => fun p => lcx{{ p }} /\ q
-  | LAndR _ q lcx => fun p => q /\ lcx{{ p }}
-  | LOrL _ lcx q  => fun p => lcx{{ p }} \/ q
-  | LOrR _ q lcx  => fun p => q \/ lcx{{ p }}
-  | LImpL _ rcx q => fun p => rcx[[ p ]] -> q
-  | LImpR _ q lcx => fun p => q -> lcx{{ p }}
-  | LAll a _ lcx  => fun p => forall (x : a), (lcx x){{ (p x) }}
-  | LEx a _ lcx   => fun p => exists (x : a), (lcx x){{ (p x) }}
-  end
-where "R [[ P ]]" := (@rcx_place _ R P) : type_scope
-and   "L {{ P }}" := (@lcx_place _ L P) : type_scope.
+where "Cx [[ P ]]" := (@ctx_place _ _ Cx P) : type_scope.
 
 Fixpoint ho_impl (Ts : list Type) : (Ts ▷ Prop) -> (Ts ▷ Prop) -> (Ts ▷ Prop) :=
   match Ts with
@@ -138,22 +121,19 @@ End HONotations.
 Import HONotations.
 
 Theorem
-  placement_r Ts (R : rcx Ts) (p q : Ts ▷ Prop) :
-    (p ⊢ q) -> R[[ p ]] -> R[[ q ]]
-with
-  placement_l Ts (L : lcx Ts) (p q : Ts ▷ Prop) :
-    (p ⊢ q) -> L{{ q }} -> L{{ p }}.
+  placement side Ts (R : ctx side Ts) (p q : Ts ▷ Prop) :
+    match side with
+    | Pos => (p ⊢ q) -> R[[ p ]] -> R[[ q ]]
+    | Neg => (p ⊢ q) -> R[[ q ]] -> R[[ p ]]
+    end.
 Proof.
-- induction R ; intros Hpq Hin ; try (compute in Hpq ; tauto) ;
-    cbn in Hin |- * ; try (specialize (IHR _ _ Hpq) ; try tauto).
-  * exact (fun Hq => Hin (placement_l _ _ _ _ Hpq Hq)).
+  induction R ; try destruct side0 ; intros Hpq Hin ;
+  try (compute in Hpq ; tauto) ;
+  cbn in Hin |- * ; try (specialize (IHR _ _ Hpq) ; try tauto).
+  * exact (fun x => H x _ _ (Hpq x) (Hin x)).
   * exact (fun x => H x _ _ (Hpq x) (Hin x)).
   * destruct Hin as (x & Hin) ; exists x ; exact (H x _ _ (Hpq x) Hin).
-- induction L ; intros Hqp Hin ; try (compute in Hqp ; tauto) ;
-    cbn in Hin |- * ; try (specialize (IHL _ _ Hqp) ; tauto).
-  * exact (fun Hp => Hin (placement_r _ _ _ _ Hqp Hp)).
-  * exact (fun x => H x _ _ (Hqp x) (Hin x)).
-  * destruct Hin as (x & Hin) ; exists x ; exact (H x _ _ (Hqp x) Hin).
+  * destruct Hin as (x & Hin) ; exists x ; exact (H x _ _ (Hpq x) Hin).
 Qed.
 
 Fixpoint ho_apply (Ts : list Type) U R : (U -> (Ts ▷ R)) -> (Ts ▷ U) -> (Ts ▷ R) :=
@@ -171,78 +151,45 @@ Require Import List.
 
 Definition path := list nat.
 
-Inductive resolve_r : forall Ts, Prop -> path -> rcx Ts -> (Ts ▷ Prop) -> Prop :=
+Inductive resolve : forall side Ts, Prop -> path -> ctx side Ts -> (Ts ▷ Prop) -> Prop :=
 | AtHere a :
-    resolve_r _ a nil Hole a
-| RAnd1 T path rcx a b f :
-    resolve_r _ a path rcx f ->
-    resolve_r _ (a /\ b) (0 :: path) (RAndL T rcx b) f
-| RAnd2 T path rcx a b f :
-    resolve_r _ b path rcx f ->
-    resolve_r _ (a /\ b) (1 :: path) (RAndR T a rcx) f
-| ROr1 T path rcx a b f :
-    resolve_r _ a path rcx f ->
-    resolve_r _ (a \/ b) (0 :: path) (ROrL T rcx b) f
-| ROr2 T path rcx a b f :
-    resolve_r _ b path rcx f ->
-    resolve_r _ (a \/ b) (1 :: path) (ROrR T a rcx) f
-| RImp1 T path lcx (a b : Prop) f :
-    resolve_l _ a path lcx f ->
-    resolve_r _ (a -> b) (0 :: path) (RImpL T lcx b) f
-| RImp2 T path rcx (a b : Prop) f :
-    resolve_r _ b path rcx f ->
-    resolve_r _ (a -> b) (1 :: path) (RImpR T a rcx) f
-| RAll0 A T path rcx a f :
-    (forall x, resolve_r _ (a x) path (rcx x) (f x)) ->
-    resolve_r _ (forall x, a x) (0 :: path) (RAll A T rcx) f
-| REx0 A T path rcx a f :
-    (forall x, resolve_r _ (a x) path (rcx x) (f x)) ->
-    resolve_r _ (exists x, a x) (0 :: path) (REx A T rcx) f
-with resolve_l : forall Ts, Prop -> path -> lcx Ts -> (Ts ▷ Prop) -> Prop :=
-| LAnd1 T path lcx a b f :
-    resolve_l _ a path lcx f ->
-    resolve_l _ (a /\ b) (0 :: path) (LAndL T lcx b) f
-| LAnd2 T path lcx a b f :
-    resolve_l _ b path lcx f ->
-    resolve_l _ (a /\ b) (1 :: path) (LAndR T a lcx) f
-| LOr1 T path lcx a b f :
-    resolve_l _ a path lcx f ->
-    resolve_l _ (a \/ b) (0 :: path) (LOrL T lcx b) f
-| LOr2 T path lcx a b f :
-    resolve_l _ b path lcx f ->
-    resolve_l _ (a \/ b) (1 :: path) (LOrR T a lcx) f
-| LImp1 T path rcx (a b : Prop) f :
-    resolve_r _ a path rcx f ->
-    resolve_l _ (a -> b) (0 :: path) (LImpL T rcx b) f
-| LImp2 T path lcx (a b : Prop) f :
-    resolve_l _ b path lcx f ->
-    resolve_l _ (a -> b) (1 :: path) (LImpR T a lcx) f
-| LAll0 A T path lcx a f :
-    (forall x, resolve_l _ (a x) path (lcx x) (f x)) ->
-    resolve_l _ (forall x, a x) (0 :: path) (LAll A T lcx) f
-| LEx0 A T path lcx a f :
-    (forall x, resolve_l _ (a x) path (lcx x) (f x)) ->
-    resolve_l _ (exists x, a x) (0 :: path) (LEx A T lcx) f.
+    resolve Pos _ a nil Hole a
+| And1 side Ts path ctx a b f :
+    resolve side Ts a path ctx f ->
+    resolve side Ts (a /\ b) (0 :: path) (@AndL side Ts ctx b) f
+| And2 side Ts path ctx a b f :
+    resolve side Ts b path ctx f ->
+    resolve side Ts (a /\ b) (1 :: path) (@AndR side Ts a ctx) f
+| Or1 side Ts path ctx a b f :
+    resolve side Ts a path ctx f ->
+    resolve side Ts (a \/ b) (0 :: path) (@OrL side Ts ctx b) f
+| Or2 side Ts path ctx a b f :
+    resolve side Ts b path ctx f ->
+    resolve side Ts (a \/ b) (1 :: path) (@OrR side Ts a ctx) f
+| Imp1 side Ts path ctx (a b : Prop) f :
+    resolve (flip side) Ts a path ctx f ->
+    resolve side Ts (a -> b) (0 :: path) (@ImpL side Ts ctx b) f
+| Imp2 side Ts path ctx (a b : Prop) f :
+    resolve side Ts b path ctx f ->
+    resolve side Ts (a -> b) (1 :: path) (@ImpR side Ts a ctx) f
+| All0 A side Ts path ctx a f :
+    (forall x, resolve side Ts (a x) path (ctx x) (f x)) ->
+    resolve side (A :: Ts) (forall x, a x) (0 :: path) (@AllD A side Ts ctx) f
+| Ex0 A side Ts path ctx a f :
+    (forall x, resolve side Ts (a x) path (ctx x) (f x)) ->
+    resolve side (A :: Ts) (exists x, a x) (0 :: path) (@ExD A side Ts ctx) f
+.
 
 Require Import Relation_Definitions Setoid.
 Require Import Coq.Program.Equality.
 
-Lemma
-  resolve_place_r Ts (rp : path) (rcx : rcx Ts) (a : Prop) (f : Ts ▷ Prop) :
-    resolve_r _ a rp rcx f -> rcx[[ f ]] <-> a
-with
-  resolve_place_l Ts (lp : path) (lcx : lcx Ts) (a : Prop) (f : Ts ▷ Prop) :
-    resolve_l _ a lp lcx f -> lcx{{ f }} <-> a.
+Lemma resolve_place side Ts (rp : path) (ctx : ctx side Ts) (a : Prop) (f : Ts ▷ Prop) :
+  resolve side Ts a rp ctx f -> ctx[[ f ]] <-> a.
 Proof.
-- induction 1 ; cbn ;
+  induction 1 ; cbn ;
   try match goal with
     | [ H : (forall _, _ <-> _) |- _ ] => setoid_rewrite H
-    | [ H : resolve_l _ _ _ _ _ |- _ ] => rewrite (resolve_place_l _ _ _ _ _ H)
-    end ; tauto.
-- induction 1 ; cbn ;
-  try match goal with
-    | [ H : (forall _, _ <-> _) |- _ ] => setoid_rewrite H
-    | [ H : resolve_r _ _ _ _ _ |- _ ] => rewrite (resolve_place_r _ _ _ _ _ H)
+    | [ H : resolve _ _ _ _ _ _ |- _ ] => rewrite (resolve_place _ _ _ _ _ _ H)
     end ; tauto.
 Qed.
 
@@ -309,230 +256,230 @@ Fixpoint check (deriv : deriv) (goal : Prop) : Prop :=
       let (rule, path) := rp in
       match rule with
       | RN_goal_ts_and_l =>
-          exists T rcx a b c,
-          resolve_r T goal path rcx (a → (b ∧ c))
+          exists Ts rcx a b c,
+          resolve Pos Ts goal path rcx (a → (b ∧ c))
           /\ check deriv (rcx[[ (a → b) ∧ c ]])
       | RN_goal_ts_and_r =>
           (* (c /\ (a -> b)) -> (a -> (c /\ b)) *)
-          exists T rcx a b c,
-          resolve_r T goal path rcx (a → (c ∧ b))
+          exists Ts rcx a b c,
+          resolve Pos Ts goal path rcx (a → (c ∧ b))
           /\ check deriv (rcx[[ c ∧ (a → b) ]])
       | RN_goal_and_ts_l =>
           (* (a -> b) -> (a /\ c -> b) *)
-          exists T rcx a b c,
-          resolve_r T goal path rcx ((a ∧ c) → b)
+          exists Ts rcx a b c,
+          resolve Pos Ts goal path rcx ((a ∧ c) → b)
           /\ check deriv (rcx[[ a → b ]])
       | RN_goal_and_ts_r =>
           (* (a -> b) -> (c /\ a -> b) *)
-          exists T rcx a b c,
-          resolve_r T goal path rcx ((c ∧ a) → b)
+          exists Ts rcx a b c,
+          resolve Pos Ts goal path rcx ((c ∧ a) → b)
           /\ check deriv (rcx[[ a → b ]])
       | RN_goal_ts_or_l =>
           (* (a -> b) -> (a -> b \/ c) *)
-          exists T rcx a b c,
-          resolve_r T goal path rcx (a → (b ∨ c))
+          exists Ts rcx a b c,
+          resolve Pos Ts goal path rcx (a → (b ∨ c))
           /\ check deriv (rcx[[ a → b ]])
       | RN_goal_ts_or_r =>
           (* (a -> b) -> (a -> c \/ b) *)
-          exists T rcx a b c,
-          resolve_r T goal path rcx (a → (c ∨ b))
+          exists Ts rcx a b c,
+          resolve Pos Ts goal path rcx (a → (c ∨ b))
           /\ check deriv (rcx[[ a → b ]])
       | RN_goal_or_ts =>
           (* ((a -> c) /\ (b -> c)) -> (a \/ b -> c) *)
-          exists T rcx a b c,
-          resolve_r T goal path rcx ((a ∨ b) → c)
+          exists Ts rcx a b c,
+          resolve Pos Ts goal path rcx ((a ∨ b) → c)
           /\ check deriv (rcx[[ (a → c) ∧ (b → c) ]])
       | RN_goal_ts_imp_l =>
           (* (a /\ b -> c) -> (a -> b -> c) *)
-          exists T rcx a b c,
-          resolve_r T goal path rcx (a → b → c)
+          exists Ts rcx a b c,
+          resolve Pos Ts goal path rcx (a → b → c)
           /\ check deriv (rcx[[ (a ∧ b) → c ]])
       | RN_goal_ts_imp_r =>
           (* (c -> a -> b) -> (a -> c -> b) *)
-          exists T rcx a b c,
-          resolve_r T goal path rcx (a → (c → b))
+          exists Ts rcx a b c,
+          resolve Pos Ts goal path rcx (a → (c → b))
           /\ check deriv (rcx[[ c → (a → b) ]])
       | RN_goal_imp_ts =>
           (* (c /\ (a -> b)) -> ((c -> a) -> b) *)
-          exists T rcx a b c,
-          resolve_r T goal path rcx ((c → a) → b)
+          exists Ts rcx a b c,
+          resolve Pos Ts goal path rcx ((c → a) → b)
           /\ check deriv (rcx[[ c ∧ (a → b) ]])
       | RN_goal_ts_all =>
           (* (forall x, a -> p x) -> (a -> forall x, p x) *)
-          exists T U rcx a p,
-          resolve_r T goal path rcx (a → (∀ (x : U), p x))
+          exists Ts U rcx a p,
+          resolve Pos Ts goal path rcx (a → (∀ (x : U), p x))
           /\ check deriv (rcx[[ ∀ (x : U), (a → p x) ]])
       | RN_goal_all_ts =>
           (* (exists x, p x -> b) -> (forall x, p x) -> b *)
-          exists T U rcx b p,
-          resolve_r T goal path rcx ((∀ (x : U), p x) → b)
+          exists Ts U rcx b p,
+          resolve Pos Ts goal path rcx ((∀ (x : U), p x) → b)
           /\ check deriv (rcx[[ ∃ (x : U), (p x → b) ]])
       | RN_goal_ts_ex =>
           (* (exists x, a -> p x) -> (a -> exists x, p x) *)
-          exists T U rcx a p,
-          resolve_r T goal path rcx (a → (∃ (x : U), p x))
+          exists Ts U rcx a p,
+          resolve Pos Ts goal path rcx (a → (∃ (x : U), p x))
           /\ check deriv (rcx[[ ∃ (x : U), (a → p x) ]])
       | RN_goal_ex_ts =>
           (* (forall x, p x -> a) -> (exists x, p x) -> a *)
-          exists T U rcx b p,
-          resolve_r T goal path rcx ((∃ (x : U), p x) → b)
+          exists Ts U rcx b p,
+          resolve Pos Ts goal path rcx ((∃ (x : U), p x) → b)
           /\ check deriv (rcx[[ ∀ (x : U), (p x → b) ]])
       | RN_asms_and_l_l =>
           (* (a /\ (b /\ c)) -> (a /\ b) *)
-          exists T lcx a b c,
-          resolve_l T goal path lcx (a ∧ (b ∧ c))
-          /\ check deriv (lcx{{ a ∧ b }})
+          exists Ts ctx a b c,
+          resolve Neg Ts goal path ctx (a ∧ (b ∧ c))
+          /\ check deriv (ctx[[ a ∧ b ]])
       | RN_asms_and_l_r =>
           (* (a /\ (c /\ b)) -> (a /\ b) *)
-          exists T lcx a b c,
-          resolve_l T goal path lcx (a ∧ (c ∧ b))
-          /\ check deriv (lcx{{ a ∧ b }})
+          exists Ts ctx a b c,
+          resolve Neg Ts goal path ctx (a ∧ (c ∧ b))
+          /\ check deriv (ctx[[ a ∧ b ]])
       | RN_asms_and_r_l =>
           (* ((a /\ c) /\ b) -> (a /\ b) *)
-          exists T lcx a b c,
-          resolve_l T goal path lcx ((a ∧ c) ∧ b)
-          /\ check deriv (lcx{{ a ∧ b }})
+          exists Ts ctx a b c,
+          resolve Neg Ts goal path ctx ((a ∧ c) ∧ b)
+          /\ check deriv (ctx[[ a ∧ b ]])
       | RN_asms_and_r_r =>
           (* ((c /\ a) /\ b) -> (a /\ b) *)
-          exists T lcx a b c,
-          resolve_l T goal path lcx ((c ∧ a) ∧ b)
-          /\ check deriv (lcx{{ a ∧ b }})
+          exists Ts ctx a b c,
+          resolve Neg Ts goal path ctx ((c ∧ a) ∧ b)
+          /\ check deriv (ctx[[ a ∧ b ]])
       | RN_asms_or_l_l =>
           (* (a /\ (b \/ c)) -> ((a /\ b) \/ c) *)
-          exists T lcx a b c,
-          resolve_l T goal path lcx (a ∧ (b ∨ c))
-          /\ check deriv (lcx{{ (a ∧ b) ∨ c }})
+          exists Ts ctx a b c,
+          resolve Neg Ts goal path ctx (a ∧ (b ∨ c))
+          /\ check deriv (ctx[[ (a ∧ b) ∨ c ]])
       | RN_asms_or_l_r =>
           (* (a /\ (c \/ b)) -> (c \/ (a /\ b)) *)
-          exists T lcx a b c,
-          resolve_l T goal path lcx (a ∧ (c ∨ b))
-          /\ check deriv (lcx{{ c ∨ (a ∧ b) }})
+          exists Ts ctx a b c,
+          resolve Neg Ts goal path ctx (a ∧ (c ∨ b))
+          /\ check deriv (ctx[[ c ∨ (a ∧ b) ]])
       | RN_asms_or_r_l =>
           (* ((a \/ c) /\ b) -> ((a /\ b) \/ c) *)
-          exists T lcx a b c,
-          resolve_l T goal path lcx ((a ∨ c) ∧ b)
-          /\ check deriv (lcx{{ (a ∧ b) ∨ c }})
+          exists Ts ctx a b c,
+          resolve Neg Ts goal path ctx ((a ∨ c) ∧ b)
+          /\ check deriv (ctx[[ (a ∧ b) ∨ c ]])
       | RN_asms_or_r_r =>
           (* ((c \/ a) /\ b) -> (c \/ (a /\ b)) *)
-          exists T lcx a b c,
-          resolve_l T goal path lcx ((c ∨ a) ∧ b)
-          /\ check deriv (lcx{{ c ∨ (a ∧ b) }})
+          exists Ts ctx a b c,
+          resolve Neg Ts goal path ctx ((c ∨ a) ∧ b)
+          /\ check deriv (ctx[[ c ∨ (a ∧ b) ]])
       | RN_asms_imp_l_l =>
           (* (a /\ (b -> c)) -> ((a -> b) -> c) *)
-          exists T lcx a b c,
-          resolve_l T goal path lcx (a ∧ (b → c))
-          /\ check deriv (lcx{{ (a → b) → c }})
+          exists Ts ctx a b c,
+          resolve Neg Ts goal path ctx (a ∧ (b → c))
+          /\ check deriv (ctx[[ (a → b) → c ]])
       | RN_asms_imp_l_r =>
           (* (a /\ (c -> b)) -> (c -> (a /\ b)) *)
-          exists T lcx a b c,
-          resolve_l T goal path lcx (a ∧ (c → b))
-          /\ check deriv (lcx{{ c → (a ∧ b) }})
+          exists Ts ctx a b c,
+          resolve Neg Ts goal path ctx (a ∧ (c → b))
+          /\ check deriv (ctx[[ c → (a ∧ b) ]])
       | RN_asms_imp_r_l =>
           (* ((a -> c) /\ b) -> ((b -> a) -> c) *)
-          exists T lcx a b c,
-          resolve_l T goal path lcx ((a → c) ∧ b)
-          /\ check deriv (lcx{{ (b → a) → c }})
+          exists Ts ctx a b c,
+          resolve Neg Ts goal path ctx ((a → c) ∧ b)
+          /\ check deriv (ctx[[ (b → a) → c ]])
       | RN_asms_imp_r_r =>
           (* ((c -> a) /\ b) -> (c -> (a /\ b)) *)
-          exists T lcx a b c,
-          resolve_l T goal path lcx ((c → a) ∧ b)
-          /\ check deriv (lcx{{ c → (a ∧ b) }})
+          exists Ts ctx a b c,
+          resolve Neg Ts goal path ctx ((c → a) ∧ b)
+          /\ check deriv (ctx[[ c → (a ∧ b) ]])
       | RN_asms_all_l =>
           (* (a /\ forall x, p x) -> forall x, (a /\ p x) *)
-          exists T U lcx a p,
-          resolve_l T goal path lcx (a ∧ (∀ (x : U), p x))
-          /\ check deriv (lcx{{ ∀ (x : U), (a ∧ p x) }})
+          exists Ts U ctx a p,
+          resolve Neg Ts goal path ctx (a ∧ (∀ (x : U), p x))
+          /\ check deriv (ctx[[ ∀ (x : U), (a ∧ p x) ]])
       | RN_asms_all_r =>
           (* ((forall x, p x) /\ a) -> forall x, (p x /\ a) *)
-          exists T U lcx a p,
-          resolve_l T goal path lcx ((∀ (x : U), p x) ∧ a)
-          /\ check deriv (lcx{{ ∀ (x : U), (p x ∧ a) }})
+          exists Ts U ctx a p,
+          resolve Neg Ts goal path ctx ((∀ (x : U), p x) ∧ a)
+          /\ check deriv (ctx[[ ∀ (x : U), (p x ∧ a) ]])
       | RN_asms_ex_l =>
           (* (a /\ exists x, p x) -> exists x, (a /\ p x) *)
-          exists T U lcx a p,
-          resolve_l T goal path lcx (a ∧ (∃ (x : U), p x))
-          /\ check deriv (lcx{{ ∃ (x : U), (a ∧ p x) }})
+          exists Ts U ctx a p,
+          resolve Neg Ts goal path ctx (a ∧ (∃ (x : U), p x))
+          /\ check deriv (ctx[[ ∃ (x : U), (a ∧ p x) ]])
       | RN_asms_ex_r =>
           (* ((exists x, p x) /\ a) -> exists x, (p x /\ a) *)
-          exists T U lcx a p,
-          resolve_l T goal path lcx ((∃ (x : U), p x) ∧ a)
-          /\ check deriv (lcx{{ ∃ (x : U), (p x ∧ a) }})
+          exists Ts U ctx a p,
+          resolve Neg Ts goal path ctx ((∃ (x : U), p x) ∧ a)
+          /\ check deriv (ctx[[ ∃ (x : U), (p x ∧ a) ]])
       | RN_contract =>
           (* (a -> a -> b) -> (a -> b) *)
-          exists T rcx a b,
-          resolve_r T goal path rcx (a → b)
+          exists Ts rcx a b,
+          resolve Pos Ts goal path rcx (a → b)
           /\ check deriv (rcx[[ a → (a → b) ]])
       | RN_weaken =>
           (* b -> (a -> b) *)
-          exists T rcx a b,
-          resolve_r T goal path rcx (a → b)
+          exists Ts rcx a b,
+          resolve Pos Ts goal path rcx (a → b)
           /\ check deriv (rcx[[ b ]])
       | RN_inst_r tx =>
           (* p t -> (exists x, p x) *)
-          exists T rcx U a (t : T ▷ U),
-          resolve_r T goal path rcx (∃ (x : U), a x)
+          exists Ts rcx U a (t : Ts ▷ U),
+          resolve Pos Ts goal path rcx (∃ (x : U), a x)
           /\ tx ~= t
           /\ check deriv (rcx[[ a ◆ t ]])
       | RN_inst_l tx =>
           (* (forall x, p x) -> p t *)
-          exists T lcx U a (t : T ▷ U),
-          resolve_l T goal path lcx (∀ (x : U), a x)
+          exists Ts ctx U a (t : Ts ▷ U),
+          resolve Neg Ts goal path ctx (∀ (x : U), a x)
           /\ tx ~= t
-          /\ check deriv (lcx{{ a ◆ t }})
+          /\ check deriv (ctx[[ a ◆ t ]])
       | RN_simp_imp_true =>
           (* True -> a -> True *)
-          exists T rcx a,
-          resolve_r T goal path rcx (a → ⊤)
+          exists Ts rcx a,
+          resolve Pos Ts goal path rcx (a → ⊤)
           /\ check deriv (rcx[[ ⊤ ]])
       | RN_simp_true_imp_r =>
           (* a -> (True -> a) *)
-          exists T rcx a,
-          resolve_r T goal path rcx (⊤ → a)
+          exists Ts rcx a,
+          resolve Pos Ts goal path rcx (⊤ → a)
           /\ check deriv (rcx[[ a ]])
       | RN_simp_true_imp_l =>
           (* (True -> a) -> a *)
-          exists T lcx a,
-          resolve_l T goal path lcx (⊤ → a)
-          /\ check deriv (lcx{{ a }})
+          exists Ts ctx a,
+          resolve Neg Ts goal path ctx (⊤ → a)
+          /\ check deriv (ctx[[ a ]])
       | RN_simp_false_imp =>
           (* True -> (False -> a) *)
-          exists T rcx a,
-          resolve_r T goal path rcx (⊥ → a)
+          exists Ts rcx a,
+          resolve Pos Ts goal path rcx (⊥ → a)
           /\ check deriv (rcx[[ ⊤ ]])
       | RN_simp_and_true_l =>
           (* a -> (a /\ True) *)
-          exists T rcx a,
-          resolve_r T goal path rcx (a ∧ ⊤)
+          exists Ts rcx a,
+          resolve Pos Ts goal path rcx (a ∧ ⊤)
           /\ check deriv (rcx[[ a ]])
       | RN_simp_and_true_r =>
           (* a -> (True /\ a) *)
-          exists T rcx a,
-          resolve_r T goal path rcx (⊤ ∧ a)
+          exists Ts rcx a,
+          resolve Pos Ts goal path rcx (⊤ ∧ a)
           /\ check deriv (rcx[[ a ]])
       | RN_simp_or_true_l =>
           (* True -> (a \/ True) *)
-          exists T rcx a,
-          resolve_r T goal path rcx (a ∨ ⊤)
+          exists Ts rcx a,
+          resolve Pos Ts goal path rcx (a ∨ ⊤)
           /\ check deriv (rcx[[ ⊤ ]])
       | RN_simp_or_true_r =>
           (* True -> (True \/ a) *)
-          exists T rcx a,
-          resolve_r T goal path rcx (⊤ ∨ a)
+          exists Ts rcx a,
+          resolve Pos Ts goal path rcx (⊤ ∨ a)
           /\ check deriv (rcx[[ ⊤ ]])
       | RN_simp_all_true =>
           (* True -> forall (_ : T), True *)
-          exists T U rcx,
-          resolve_r T goal path rcx (∀ (x : U), ⊤)
+          exists Ts U rcx,
+          resolve Pos Ts goal path rcx (∀ (x : U), ⊤)
           /\ check deriv (rcx[[ ⊤ ]])
       | RN_init =>
           (* True -> p -> p *)
-          exists T rcx p,
-          resolve_r T goal path rcx (p → p)
+          exists Ts rcx p,
+          resolve Pos Ts goal path rcx (p → p)
           /\ check deriv (rcx[[ ⊤ ]])
       | RN_congr =>
           (* True -> t = t *)
-          exists T rcx A (t : T ▷ A),
-          resolve_r T goal path rcx (t ≐ t)
+          exists Ts rcx A (t : Ts ▷ A),
+          resolve Pos Ts goal path rcx (t ≐ t)
           /\ check deriv (rcx[[ ⊤ ]])
       end
   end.
@@ -546,14 +493,14 @@ Proof.
               cbn in Hcheck ; destruct Hcheck
           | [ H : ex _ |- _ ] => destruct H
           | [ H : _ /\ _ |- _ ] => destruct H
-          | [ H : resolve_r _ _ _ _ _, Hch : check _ _ |- _ ] =>
+          | [ H : resolve Pos _ _ _ _ _, Hch : check _ _ |- _ ] =>
               specialize (IHderiv _ Hch) ;
-              rewrite <- (resolve_place_r _ _ _ _ _ H) ;
-              refine (placement_r _ _ _ _ _ IHderiv)
-          | [ H : resolve_l _ _ _ _ _, Hch : check _ _ |- _ ] =>
+              rewrite <- (resolve_place Pos _ _ _ _ _ H) ;
+              refine (placement Pos _ _ _ _ _ IHderiv)
+          | [ H : resolve Neg _ _ _ _ _, Hch : check _ _ |- _ ] =>
               specialize (IHderiv _ Hch) ;
-              rewrite <- (resolve_place_l _ _ _ _ _ H) ;
-              refine (placement_l _ _ _ _ _ IHderiv)
+              rewrite <- (resolve_place Neg _ _ _ _ _ H) ;
+              refine (placement Neg _ _ _ _ _ IHderiv)
           | [ |- ho_entails ?x _ _ ] =>
               let Ts := fresh "Ts" in
               rename x into Ts ; clear ; induction Ts as [ | A Ts ] ;
